nfa

NFA.v
@@ -1,69 +1,74 @@
 
-Require Export Str.
+Require Export Str Reg.
 
 
 
-Section NFA.
 
 
-Record sym : Type := mkSym {
-    symb :> finStr;
-    _ : symb ∈ ([set [::x]| x in [set : symbol]] ∪ [set ϵ]);
+Record chars {finStr : str}: Type := mkChar {
+    c :> finStr;
+    _ : c ∈ ([set [::x]| x in [set : char]] ∪ [set ϵ]);
 }.
 
 
 
-Definition ϵ_ : sym.
-    apply (mkSym nil).
+Definition ϵ_ {finStr : str}: chars.
+    apply (mkChar _ ϵ).
     rewrite inE; apply /orP; right.
     rewrite inE => //.
 Qed.
 
-Definition toSym (a : symbol) : sym.
+Definition charOf {finStr : str} (a : char) : chars.
 Proof.
-    apply (mkSym [:: a]).
+    apply (mkChar _ [:: a]).
     rewrite inE; apply /orP; left.
     apply /imsetP; exists a => //.
 Qed.
 
-
-Variable state : finType.
-Variables Q F : {set state}.
-Hypotheses FQ : F ⊂ Q.
-Variable p0 : state.
-Hypotheses pQ : p0 ∈ Q.
-Variable δ : state -> sym ->  {set state}.
-
-
+Class nfa {finStr : str} : Type := mkNFA {
+    state : finType;
+    Q : {set state};
+    F : {set state};
+    p0 : state;
+    δ : state -> chars -> {set state}
+}.
 
 
 
 
 Reserved Notation "p -ϵ-> q"(at level 50).
-Inductive Closure : state -> state -> Prop :=
+Inductive Closure {finStr : str} {N : nfa}: state -> state -> Prop :=
     | CL_refl p : p -ϵ-> p
     | CL_single p q : q ∈ δ p ϵ_ -> p -ϵ-> q
     | CL_trans p q r : p -ϵ-> q -> q -ϵ-> r ->  p -ϵ-> r
     where "p -ϵ-> q" := (Closure p q).
 
-Axiom closure : {set state} -> {set state}.
-Axiom closureP : forall (P : {set state}) q,
+Axiom closure : forall {finStr : str} {N : nfa}, {set state} -> {set state}.
+Axiom closureP : forall {finStr : str} {N : nfa} (P : {set state}) q,
     reflect (forall p, p ∈ P -> p -ϵ-> q) (q ∈ closure P).
 
 
-
-
-
-Fixpoint δ' (p : state) (s : finStr) : {set state} :=
+Fixpoint δ' {finStr : str} {N : nfa} (p : state) (s : finStr) : {set state} :=
     match s with
     | [::] => closure [set p]
-    | a :: w => closure (bigcup [set δ x (toSym a) | x in δ' p w])
+    | a :: w => closure (bigcup [set δ x (charOf a) | x in δ' p w])
     end.
 
-Definition L := [set w : finStr | (δ' p0 w ∩ F) == ∅].
+Definition L {finStr : str} (N : nfa) := [set w : finStr | (δ' p0 w ∩ F) == ∅].
 
 
-End NFA.
+
+
+Section Properties.
+
+Context (finStr : str) (lo : lang_op finStr)(Σ : lang).
+
+Theorem reg_nfa :
+    forall l : Σ, Reg l -> exists N : nfa, L N = l.
+Proof.
+Admitted.
+
+
 
  
 
